LeanScratch/Computation/RegTree.lean
@@ -7,16 +7,18 @@ inductive RegTree
   | lf (n : Nat)
   | br (l r : RegTree)
 
-abbrev RegTree.toStore : RegTree → Type
-  | .lf n => Vec Nat n
-  | .br l r => l.toStore × r.toStore
-
 def Vec.zero {n} : Vec Nat n :=
   match n with
   | 0 => %[]
   | _+1 => 0 %::zero
 
-def RegTree.toStore.zero {r : RegTree} : r.toStore :=
+namespace RegTree
+
+abbrev toStore : RegTree → Type
+  | .lf n => Vec Nat n
+  | .br l r => l.toStore × r.toStore
+
+def toStore.zero {r : RegTree} : r.toStore :=
   match r with
   | .lf _ => Vec.zero
   | .br _ _ => ⟨zero, zero⟩
@@ -28,6 +30,164 @@ instance {r : RegTree} : Repr r.toStore where
       | .lf _ => repr v
       | .br _ _ => .bracket "⟨" (f v.fst ++ ", " ++ f v.snd) "⟩"
 
-abbrev RegTree.toIdx : RegTree → Type
+abbrev toIdx : RegTree → Type
   | .lf n => Fin2 n
   | .br l r => l.toIdx ⊕ r.toIdx
+
+instance instDecEq {r : RegTree} : DecidableEq r.toIdx := match r with
+  | .lf n => Fin2.decEq
+  | .br l r => fun
+    | .inl a, .inl b
+    | .inr a, .inr b =>
+      match instDecEq a b with
+      | .isTrue  p => .isTrue $ p.rec rfl
+      | .isFalse p => .isFalse fun x => by
+        injections x
+        exact p x
+    | .inl _, .inr _ | .inr _, .inl _ => .isFalse Sum.noConfusion
+
+instance instFintype2 {r : RegTree} : Fintype2 (r.toIdx) := match r with
+  | .lf n => Fin2.instFintype2
+  | .br l r => {
+    elems :=
+      (instFintype2 (r := l)).elems.map Sum.inl ++
+      (instFintype2 (r := r)).elems.map Sum.inr
+    complete := fun | .inl _ | .inr _ => by simp [instFintype2.complete]
+    nodup :=
+      List.nodup_append.mpr ⟨
+        List.Nodup.map (@Sum.inl.inj _ _) instFintype2.nodup,
+        List.Nodup.map (@Sum.inr.inj _ _) instFintype2.nodup,
+        by simp [List.Disjoint]⟩
+  }
+  /- elems := match r with -/
+  /-   | .lf n => (Fin2.instFintype n).elems -/
+  /-   | .br l r => sorry -/
+  /- complete := sorry -/
+
+abbrev lookup (r : RegTree) (store : r.toStore) (idx : r.toIdx) : Nat :=
+  match r with
+  | .lf _ => store.lookup idx
+  | .br _ _ =>
+    match idx with
+    | .inl idx => RegTree.lookup _ store.fst idx
+    | .inr idx => RegTree.lookup _ store.snd idx
+
+def set (r : RegTree) (store : r.toStore) (idx : r.toIdx) (v : Nat) : r.toStore :=
+  match r, idx, store with
+  | .lf _, idx, s => s.set idx v
+  | .br l _, .inl idx, ⟨sl, sr⟩ => ⟨l.set sl idx v, sr⟩
+  | .br _ r, .inr idx, ⟨sl, sr⟩ => ⟨sl, r.set sr idx v⟩
+
+theorem set.overwrite {r : RegTree} {store : r.toStore} {idx : r.toIdx}
+    : r.set (r.set store idx y) idx x = r.set store idx x :=
+  match r, idx with
+  | .lf _, idx => Vec.set.overwrite
+  | .br _ _, .inr _
+  | .br _ _, .inl _ => by
+    dsimp [set]
+    rw [set.overwrite]
+
+theorem set.comm_ne {r : RegTree} {idx jdx : r.toIdx} {s1 : r.toStore} (hNe : idx ≠ jdx)
+    : r.set (r.set s1 idx x) jdx y = r.set (r.set s1 jdx y) idx x :=
+  match r, idx, jdx with
+  | .lf _, idx, jdx => Vec.set.comm_ne hNe
+  | .br _ _, .inl x, .inr y | .br _ _, .inr x, .inl y => rfl
+  | .br l r, .inl x, .inl y | .br l r, .inr x, .inr y => by
+    dsimp [set]
+    rw [RegTree.set.comm_ne]
+    exact hNe ∘ (·.rec rfl)
+
+def set_many (r : RegTree) (store : r.toStore) : List (r.toIdx × Nat) → r.toStore
+  | [] => store
+  | ⟨idx, x⟩ :: tl => r.set (r.set_many store tl) idx x
+
+def set_many.stalin [DecidableEq T] : List (T × V) → List (T × V)
+  | [] => []
+  | ⟨k, v⟩ :: tl => ⟨k, v⟩ :: ((set_many.stalin tl).filter $ (· ≠ k) ∘ Prod.fst)
+
+-- Closer to the one-child policy (what happend to monday) than stalin
+theorem set_many.stalin.nodup
+    [DecidableEq T] {ls : List (T × V)}
+    : (set_many.stalin ls).map Prod.fst |>.Nodup :=
+  match ls with
+  | [] => .nil
+  | hd :: tl => .cons
+    (by simp [←List.filter_map, List.mem_filter])
+    (by simp [←List.filter_map, List.Nodup.filter, nodup])
+
+theorem set_many.stalin.lem {r : RegTree} {s : r.toStore} (k : r.toIdx) (v : ℕ)
+    (sub : List (r.toIdx × ℕ))
+    : r.set (r.set_many s (List.filter ((fun x ↦ decide ¬x = k) ∘ Prod.fst) sub)) k v =
+      r.set (r.set_many s sub) k v := by
+  induction sub
+  · rfl
+  case cons hd tl ih =>
+    rcases hd with ⟨hk, hv⟩
+    rw [List.filter_cons]
+    split <;> rename_i h <;> simp at h <;> dsimp [set_many]
+    · rw [RegTree.set.comm_ne h, RegTree.set.comm_ne h, ih]
+    · rw [h, RegTree.set.overwrite, ih]
+
+theorem set_many.stalin.sm
+    {r : RegTree} {s : r.toStore}
+    (ls : List (r.toIdx × Nat))
+    : r.set_many s ls = r.set_many s (stalin ls) :=
+  match ls with
+  | [] => rfl
+  | ⟨k, v⟩ :: tl => by dsimp [set_many, stalin]; rw [lem, sm]
+
+/- theorem set_many.stalin.nochange -/
+/-     {ls : List (T × U)} -/
+/-     [DecidableEq T] -/
+/-     {} -/
+/-     : set_many.stalin ls = ls := -/
+/-   sorry -/
+
+theorem set_many.comp {r : RegTree} {base : r.toStore} {l₁ l₂ : List (r.toIdx × Nat)} :
+    r.set_many (r.set_many base l₁) l₂ = r.set_many base (l₂ ++ l₁) :=
+  match l₂ with
+  | [] => rfl
+  | ⟨idx, v⟩ :: tl => by
+    dsimp [set_many]
+    rw [set_many.comp]
+
+def set_many.perm {r : RegTree} {l₁ l₂ : List (r.toIdx × Nat)}
+    {s : r.toStore}
+    (hNoDup : l₁.map Prod.fst |>.Nodup)
+    (hPerm : List.Perm l₁ l₂)
+    : r.set_many s l₁ = r.set_many s l₂ := by
+  induction hPerm generalizing s
+  case cons el _ ih =>
+    rename_i tl₁ _
+    rcases hNoDup with (_|⟨hhd, hNoDup⟩)
+    simp only [set_many]
+    rw [ih hNoDup]
+  case swap x y ls =>
+    rcases x with ⟨xk, xv⟩
+    rcases y with ⟨yk, yv⟩
+    rcases hNoDup with (_|⟨hhd, hnodup⟩)
+    simp only [List.map_cons, List.mem_cons, List.mem_map, Prod.exists, exists_and_right,
+      exists_eq_right, ne_eq, forall_eq_or_imp, forall_exists_index] at hhd
+    rcases hhd with ⟨neq, _⟩
+    dsimp [set_many]
+    rw [set.comm_ne neq]
+  case trans a _ iha ihb =>
+    calc
+      _ = _ := iha hNoDup
+      _ = _ := ihb $ (List.Perm.nodup_iff $ List.Perm.map _ a).mp hNoDup
+  case nil => rfl
+
+@[ext]
+def store.ext {r : RegTree} {s1 s2 : r.toStore}
+    (h : r.lookup s1 = r.lookup s2)
+    : s1 = s2 :=
+  match r, s1, s2 with
+  | .lf _, s1, s2 => Vec.ext h
+  | .br l r, ⟨l₁, r₁⟩, ⟨l₂, r₂⟩ => by
+    have := Function.funext_iff.mp h
+    have l : l.lookup l₁ = l.lookup l₂ := funext $ λ x ↦ this (.inl x)
+    have r : r.lookup r₁ = r.lookup r₂ := funext $ λ x ↦ this (.inr x)
+    rw [RegTree.store.ext l, RegTree.store.ext r]
+
+end RegTree
+
