LeanScratch/Computation/Subroutine.lean
@@ -1,0 +1,239 @@
+import LeanScratch.Computation.RegMachine
+
+namespace Comp
+
+variable {InsA InsB} [Fintype2 InsA] [Fintype2 InsB]
+
+def subroutine
+    {r t : RegTree}
+    (inM : RegMachine r InsA)
+    (rmapper : r.toIdx → t.toIdx)
+    (imapper : InsA → InsB)
+    (hltStepper : InsB)
+    (x : InsA)
+    : RegMachine.Ins t InsB :=
+  match inM x with
+  | .inc r next =>
+    let next := match inM next with
+      | .hlt => hltStepper
+      | _    => imapper next
+    .inc (rmapper r) next
+  | .dec r nz z =>
+    let nz := match inM nz with
+      | .hlt => hltStepper
+      | _    => imapper nz
+    let z  := match inM z with
+      | .hlt => hltStepper
+      | _    => imapper z
+    .dec (rmapper r) nz z
+  | .hlt => .hlt -- This case should be handled differently maybe
+
+theorem RegMachine.step.none_hlt [Fintype2 L] {inM : RegMachine r L}
+    (h : RegMachine.Config.step inM ⟨view, s⟩ = none)
+    : inM s = .hlt :=
+  match heq : inM s with
+  | .hlt => rfl
+  | .inc _ _ | .dec _ _ _ => by
+    simp only [Config.step, heq] at h
+    <;> split at h
+    <;> exact Option.noConfusion h
+
+def updateImageVec
+    {t : RegTree}
+    (rmapper : Fin2 n → t.toIdx)
+    (src : Vec Nat n)
+    (dst : t.toStore)
+    : t.toStore :=
+  match src with
+  | %[] => dst
+  | hd %:: tl => t.set (updateImageVec (rmapper ∘ Fin2.fs) tl dst) (rmapper .fz) hd
+
+abbrev updateImageVec_alt
+    {t : RegTree}
+    (rmapper : Fin2 n → t.toIdx)
+    (src : Vec Nat n)
+    (dst : t.toStore)
+    : t.toStore :=
+  t.set_many dst (Fin2.instFintype2.elems.map (fun x => ⟨rmapper x, src.lookup x⟩))
+
+theorem updateImageVec_eq_alt
+    {t : RegTree}
+    {rmapper : Fin2 n → t.toIdx}
+    {src : Vec Nat n}
+    {dst : t.toStore}
+    : updateImageVec rmapper src dst =
+      updateImageVec_alt rmapper src dst :=
+  match n, src with
+  | 0, %[] => by simp [updateImageVec_alt, updateImageVec, Fin2.instFintype, RegTree.set_many]
+  | n+1, hd %:: tl => by
+    set_option pp.all true in
+    dsimp [updateImageVec, updateImageVec_alt, Fintype2.elems, RegTree.set_many, Vec.lookup]
+    rw [List.map_map]
+    congr
+    change _ = updateImageVec_alt _ _ _
+    exact updateImageVec_eq_alt
+
+/- /-- error: (kernel) deep recursion detected -/ -/
+/- #guard_msgs in -/
+/- abbrev UI_alt -/
+/-     {r t : RegTree} -/
+/-     (rmapper : r.toIdx → t.toIdx) -/
+/-     (src : r.toStore) -/
+/-     (dst : t.toStore) -/
+/-     : t.toStore := -/
+/-   t.set_many dst (RegTree.instFintype2.elems.map (fun x => ⟨rmapper x, r.lookup src x⟩)) -/
+
+def updateImage
+    {r t : RegTree}
+    (rmapper : r.toIdx → t.toIdx)
+    (src : r.toStore)
+    (dst : t.toStore)
+    : t.toStore :=
+  match r, src with
+  | .lf _, v => updateImageVec rmapper v dst
+  | .br _ _, ⟨lsrc, rsrc⟩ =>
+    (updateImage (rmapper ∘ Sum.inr) rsrc dst) |>
+    (updateImage (rmapper ∘ Sum.inl) lsrc ·)
+
+theorem updateImage_eq_alt
+    {r t : RegTree}
+    {rmapper : r.toIdx → t.toIdx}
+    {src : r.toStore}
+    {dst : t.toStore}
+    : updateImage rmapper src dst =
+      t.set_many dst (RegTree.instFintype2.elems.map (fun x => ⟨rmapper x, r.lookup src x⟩)) :=
+  match r, src with
+  | .lf _, v => updateImageVec_eq_alt
+  | .br _ _, ⟨a, b⟩ => by
+    dsimp [updateImage, Fintype2.elems]
+    rw [List.map_append, List.map_map, List.map_map]
+    rw [updateImage_eq_alt, updateImage_eq_alt]
+    rw [RegTree.set_many.comp]
+    rfl
+
+theorem updateImage.comm_inj
+    {r l t : RegTree}
+    {rmapper : (r.br l).toIdx → t.toIdx}
+    {rs : r.toStore}
+    {ls : l.toStore}
+    {dst : t.toStore}
+    (hInj : Function.Injective rmapper)
+    : updateImage (rmapper ∘ Sum.inr) ls (updateImage (rmapper ∘ Sum.inl) rs dst) =
+      updateImage (rmapper ∘ Sum.inl) rs (updateImage (rmapper ∘ Sum.inr) ls dst) := by
+  rw [updateImage_eq_alt, updateImage_eq_alt, RegTree.set_many.comp, updateImage_eq_alt, updateImage_eq_alt, RegTree.set_many.comp]
+  apply RegTree.set_many.perm _ (List.perm_append_comm)
+  simp only [Function.comp_apply, List.map_append, List.map_map]
+  change List.Nodup ((List.map (rmapper ∘ Sum.inr) _) ++ (List.map (rmapper ∘ Sum.inl) _))
+  apply List.Nodup.append
+  case dj =>
+    simp only [List.Disjoint, List.mem_map, Function.comp_apply, imp_false, not_exists, not_and,
+      forall_exists_index, and_imp, forall_apply_eq_imp_iff₂]
+    exact fun _ _ _ _ h => Sum.noConfusion (hInj h)
+  all_goals apply List.Nodup.map
+  <;> (try exact Fintype2.nodup) <;> apply Function.Injective.comp hInj
+  · exact @Sum.inr.inj _ _
+  · exact @Sum.inl.inj _ _
+
+theorem updateImageVec.inc_slide
+    {t : RegTree}
+    {rmapper : Fin2 n → t.toIdx}
+    {iInitStore outerStore}
+    : RegMachine.inc (rmapper reg) (updateImageVec rmapper iInitStore outerStore) =
+      updateImageVec rmapper       (RegMachine.inc_vec reg iInitStore) outerStore :=
+  match n, iInitStore, reg with
+  | n+1, hd %:: tl, .fz => by dsimp [RegMachine.inc_vec, updateImageVec]; sorry
+  | n+1, hd %:: tl, .fs idx => by
+    simp [updateImageVec]
+    sorry
+
+/- theorem Comp.updateImage.extracted_1 -/
+/-     {r t : RegTree} {rmapper : r.toIdx → t.toIdx} {iInitStore : r.toStore} -/
+/-     {outerStore : t.toStore} {reg : r.toIdx} {x : t.toIdx} (h : x = rmapper reg) -/
+/-     : t.set (updateImage rmapper iInitStore outerStore) x (t.lookup (updateImage rmapper iInitStore outerStore) x).succ = -/
+/-       updateImage rmapper (r.set iInitStore reg (r.lookup iInitStore reg).succ) outerStore := -/
+/-   match r, t, x, reg with -/
+/-   | _, _, _, _ => sorry -/
+
+theorem updateImage.inc_slide
+    {r t : RegTree}
+    {rmapper : r.toIdx → t.toIdx}
+    {iInitStore outerStore}
+    {reg : r.toIdx}
+    : RegMachine.inc (rmapper reg) (updateImage rmapper iInitStore outerStore) =
+      updateImage rmapper (RegMachine.inc reg iInitStore) outerStore := by
+  rw [RegMachine.inc.eq_set]
+  rw [RegMachine.inc.eq_set]
+  sorry
+  /- match r, reg, iInitStore with -/
+  /- | .lf _, reg, store => sorry -/
+  /- | .br _ _, .inl reg, ⟨l, r⟩ => by -/
+  /-   dsimp [RegMachine.inc] -/
+  /-   conv => -/
+  /-     lhs; -/
+  /-     dsimp [updateImage, RegMachine.inc] -/
+  /-   /- rw [updateImage.inc_slide] -/ -/
+  /-   sorry -/
+  /- | .br _ _, .inr reg, ⟨l, r⟩ => by -/
+  /-   sorry -/
+
+theorem subroutine.forward
+    {r t : RegTree}
+    {prog : RegMachine t InsB}
+
+    {inM : RegMachine r InsA}
+    {rmapper : r.toIdx → t.toIdx}
+    {imapper : InsA → InsB}
+
+    {iInitStore iEndStore outerStore}
+
+    -- the following theorems should all be solvable with large simps
+    (hIsSub : prog ∘ imapper = subroutine inM rmapper imapper hltStepper)
+
+    (hRInj : Function.Injective rmapper)
+    (hIInj : Function.Injective imapper)
+
+    (hInTW : inM.TW ⟨iInitStore, startS⟩ ⟨iEndStore, endS⟩)
+    (hStartNotHlt : inM startS ≠ .hlt)
+
+    : prog.StepsTo ⟨updateImage rmapper iInitStore outerStore, imapper startS⟩
+                   ⟨updateImage rmapper iEndStore  outerStore, hltStepper⟩ := by
+  rcases hInTW with ⟨w, term, v⟩
+  induction w generalizing startS iInitStore
+  · obtain ⟨rfl, rfl⟩ := (RegMachine.Config.mk.injEq _ _ _ _).mp $ (Option.some.injEq _ _).mp term
+    exact (hStartNotHlt $ RegMachine.step.none_hlt v).elim
+  case succ n ih =>
+    obtain ⟨⟨imStore, imState⟩, stepper, p⟩ := Option.bind_eq_some.mp term
+    clear term
+
+    exists n+1
+    simp only [RegMachine.Config.step_n]
+    apply Option.bind_eq_some.mpr
+    dsimp [RegMachine.Config.step, subroutine]
+    simp [Function.funext_iff] at hIsSub
+    rw [hIsSub]
+    dsimp [subroutine]
+    cases heq : inM startS
+    <;> (try exact (hStartNotHlt heq).elim)
+    <;> rename_i reg nextins
+    <;> by_cases hNextEq : inM nextins = .hlt
+    · clear ih
+      use ⟨RegMachine.inc (rmapper reg) (updateImage rmapper iInitStore outerStore), hltStepper⟩
+      simp [hNextEq]
+      simp only [RegMachine.Config.step, heq, Option.some.injEq, RegMachine.Config.mk.injEq] at stepper
+      rcases stepper with ⟨rfl, rfl⟩
+      obtain rfl : n = 0 := by
+        cases n
+        · rfl
+        · simp [RegMachine.Config.step_n, RegMachine.Config.step, hNextEq] at p
+      simp_all only [ne_eq, not_false_eq_true, RegMachine.Config.step_n.zero, Option.some.injEq,
+        RegMachine.Config.mk.injEq, and_true]
+      rcases p with ⟨rfl, rfl⟩
+      sorry
+      /- by_cases hInImage : ∃ v', v = rmapper v' -/
+      /- sorry -/
+      /- · have := hNeqStores _ hInImage -/
+      /-   sorry -/
+    · sorry
+    · sorry
+    · sorry
+
